# sympy_matrix_tools

<!-- Time-stamp: "2022-05-04T12:41:22Z" -->

Some tools for SymPy matrices.

## Download in Google Colab

``` python
!pip install git+https://github.com/JRF-2018/sympy_matrix_tools
```

## Fix coeff

This module can fix a MatMul.args_cnc error like below...

``` python
>>> from sympy import *
>>> N = Symbol("N", integer=True)
>>> x1 = Symbol("x1")
>>> M1 = MatrixSymbol("M1", N, N)
>>> M2 = MatrixSymbol("M2", N, N)
>>> z = (M2 + 2 * (M2 + Identity(N)) * M1 + Identity(N))
>>> z.coeff(M1)
Traceback (most recent call last):
  ...
AttributeError: 'list' object has no attribute 'difference'

```

To fix it...

``` python
>>> import sympy_matrix_tools
>>> sympy_matrix_tools.fix_MatMul_args_cnc()
>>> z.coeff(M1)
2*I + 2*M2

```


## Usage of functions for matrices

```python
>>> from sympy_matrix_tools import *
>>> z = (M1 + M2) * M1 + 2 * x1 * (x1 + 1) * M1 * M2 + M2 * (M1 ** 2) + 3 * M2 * M1
>>> mat_coeff(z, M1)
M1 + M2
>>> mat_coeff(z, 2 * M2)
x1*(x1 + 1)*M1
>>> mat_coeff(z, M1, right=True)
2*x1*(x1 + 1)*M2
>>> mat_coeff(z, M1 + M2, right=True)
M1
>>> mat_coeff(z, M1, nth=1)
3*M2
>>> mat_coeff(z, M1 ** 2)
M2
>>> mat_coeff(z, M1, nth=1, expand_pow=True)
M2*M1

```

```python
>>> z = M1 * M2 + (M2 + M1) * M1 + (M2 + M1) * (M1 ** 2) + (M2 + M1) * M2 + 3 * M1
>>> mat_collect(z, M1)
(M1 + M2)*M1**2 + (M1 + M2)*M2 + (3*I + M1 + M2)*M1 + M1*M2
>>> mat_collect(z, M1, expand_pow=True)
(M1 + M2)*M2 + ((M1 + M2)*M1 + 3*I + M1 + M2)*M1 + M1*M2

```

```python
>> z
(M1 + M2)*M1**2 + (M1 + M2)*M1 + (M1 + M2)*M2 + 3*M1 + M1*M2
>> z.args[1]
(M1 + M2)*M1**2
>>> partial_apply(z, z.args[1], lambda y: y.expand().doit())
M1**3 + M2*M1**2 + (M1 + M2)*M1 + (M1 + M2)*M2 + 3*M1 + M1*M2

```

```python
>>> mat_divide(M1 * M2, M1)
M2
>>> mat_divide(M1 * M2, M1, right=True)
M1*M2*M1**(-1)
>>> mat_divide(M1 * M2, M2)
M2**(-1)*M1*M2
>>> mat_divide(M1 * M2, M2, right=True)
M1
>>> mat_divide(M1 * M2 + 2 * x1 * (M1 + M2) * M2, M1)
(2*x1)*M1**(-1)*(M1 + M2)*M2 + M2
>>> mat_divide(M1 * M2 + 2 * x1 * (M1 + M2) * M2, 3 * x1 * (M1 + M2))
(1/(3*x1))*(M1 + M2)**(-1)*M1*M2 + (2/3)*M2

```

Mixed Example:
```python
>>> z = M1 * M2 + (x1 ** 2) * (M2 + M1) * M1 + x1 * (M2 + M1) * (M1 ** 2) + (M2 + M1) * M2 + 3 * M1
>>> z2 = mat_collect(z, x1 * M1, expand_pow=True)
>>> z2
x1*(x1*(M1 + M2) + (M1 + M2)*M1)*M1 + (M1 + M2)*M2 + 3*M1 + M1*M2
>>> mat_coeff(z2, x1 * M1)
x1*(M1 + M2) + (M1 + M2)*M1
>>> mat_divide(z2, x1 * M1, right=True)
(3/x1)*I + x1*(M1 + M2) + (M1 + M2)*M1 + 1/x1*(M1 + M2)*M2*M1**(-1) + 1/x1*M1*M2*M1**(-1)

```

```python
>>> z = x1 ** N * M1**N + x1 * M1 ** 2
>>> z2 = mat_collect(z, x1 *  M1 ** 2, expand_pow=2)
>>> z2
x1*((x1*x1**(N - 2))*M1**(N - 2) + I)*M1**2
>>> z2.args[1]
(x1*x1**(N - 2))*M1**(N - 2) + I
>>> partial_apply(z2, z2.args[1], lambda y: y.expand().doit())
x1*((x1**N/x1)*M1**(N - 2) + I)*M1**2
>>> mat_collect(z, x1 *  M1 ** 2, expand_pow=2, expand_inner=True)
x1*((x1**N/x1)*M1**(N - 2) + I)*M1**2
>>> mat_collect(z, x1 *  M1 ** 2, expand_pow={x1**N: 1, M1**N: 2})
x1*(x1**(N - 1)*M1**(N - 2) + I)*M1**2

```


## Usage of MatrixFunction (**Experimental**)

```python
>>> N = Symbol("N", integer=True)
>>> N2 = Symbol("N2", integer=True)
>>> x1 = Symbol("x1")
>>> M1 = MatrixSymbol("M1", N + 1, N + 1)
>>> M2 = MatrixSymbol("M2", N + 1, N + 1)

```

```python
>>> Mf = MatrixFunction("Mf", N + 1, N + 1)
>>> Mf(N) + M1
Mf(N) + M1
>>> (Mf(N) + M1).subs(Mf, Lambda(x1, x1 * M1 + M2)).subs(N, 2).doit()
3*M1 + M2
>>> # The following example seems to be able to differentiate well, but it doesn't really work.
>>> (Mf(2 * x1 + 1) + M1).diff(x1)
2*Subs(Derivative(Mf(_xi_1), _xi_1), _xi_1, 2*x1 + 1) + 0
>>> (Mf(2 * x1 + 1) + M1).diff(x1) + ZeroMatrix(N+1,N+1)
Traceback (most recent call last):
  ...
AttributeError: 'Mul' object has no attribute 'shape'
>>> # However, it may work in practice.
>>> (Mf(2 * x1 + 1) + M1).diff(x1).subs(Mf, Lambda(x1, x1 * M1 + M2)).doit()
2*M1

```


## Usage of functions for sequences

```python
>>> f = Function("f")
>>> g = Function("g")
>>> n = Symbol("n", integer=True)
>>> m = Symbol("m", integer=True)
>>> m2 = Symbol("m2", integer=True)
>>> T = Symbol("T", integer=True)
>>> tau = Symbol("tau", integer=True)

```

```python
>>> z = Sum(g(m) + Sum(f(n, m), (n, 0, T)), (m, 0, tau)) + Sum(f(n, 0), (n, 0, tau))
>>> atoms_list(z, Sum)
[Sum(g(m) + Sum(f(n, m), (n, 0, T)), (m, 0, tau)), Sum(f(n, m), (n, 0, T)), Sum(f(n, 0), (n, 0, tau))]
>>> nth_Sum(z, 0)
Sum(g(m) + Sum(f(n, m), (n, 0, T)), (m, 0, tau))
>>> Sum_expand(z)
Sum(f(n, 0), (n, 0, tau)) + Sum(g(m), (m, 0, tau)) + Sum(f(n, m), (n, 0, T), (m, 0, tau))
>>> Sum_swap(Sum_expand(z))
Sum(f(n, 0), (n, 0, tau)) + Sum(g(m), (m, 0, tau)) + Sum(f(n, m), (m, 0, tau), (n, 0, T))
>>> z2 = Sum_collect(z)
>>> z2
Sum(f(_xi, 0) + g(_xi) + Sum(f(n, _xi), (n, 0, T)), (_xi, 0, tau))

```


When collectiong with level >= 2, matching the names of bound symbols is required. A bound symbol can be replaced as follows. But the example is not appropriate, because it has already been collected...

```python
>>> z = Sum(g(m) + Sum(f(n, m), (n, 0, T)), (m, 0, tau)) + Sum(f(m2, 2 * m), (m2, 0, T), (m, 0, tau))
>>> z = Sum_expand(z)
>>> z
Sum(g(m), (m, 0, tau)) + Sum(f(m2, 2*m), (m2, 0, T), (m, 0, tau)) + Sum(f(n, m), (n, 0, T), (m, 0, tau))
>>> z2 = Sum_collect(z, level=2)
>>> z2
Sum(g(m), (m, 0, tau)) + Sum(f(_xi, m) + f(_xi, 2*m), (_xi, 0, T), (m, 0, tau))
>>> xi = list(z2.atoms(Dummy))[0]
>>> z2.replace(xi, n)
Sum(g(m), (m, 0, tau)) + Sum(f(n, m) + f(n, 2*m), (n, 0, T), (m, 0, tau))

```

Partially expand symbolic series.

```python
>>> z = Sum(f(n + 1), (n, 0, T))
>>> Sum_step_forward(z)
f(1) + Sum(f(n + 1), (n, 1, T))
>>> Sum_step_forward(z, step=2)
f(1) + f(2) + Sum(f(n + 1), (n, 2, T))
>>> Sum_step_forward(z, step=2, begin=0)
f(1) + f(2) + Sum(f(n + 3), (n, 0, T - 2))
>>> Sum_step_forward(z, step=2, end=tau)
f(1) + f(2) + Sum(f(T + n - tau + 1), (n, -T + tau + 2, tau))
>>> Sum_step_forward(z, step=-2)
-f(-1) - f(0) + Sum(f(n + 1), (n, -2, T))
>>> Sum_step_backward(z)
f(T + 1) + Sum(f(n + 1), (n, 0, T - 1))
>>> Sum_step_backward(z, step=2)
f(T) + f(T + 1) + Sum(f(n + 1), (n, 0, T - 2))
>>> Sum_step_backward(z, step=-2)
-f(T + 2) - f(T + 3) + Sum(f(n + 1), (n, 0, T + 2))
>>> Sum_step_forward(z, step=tau, minus=False)
Sum(f(n + 1), (n, 0, tau)) + Sum(f(n + 1), (n, tau + 1, T))
>>> Sum_step_forward(z, step=-tau, minus=True)
Sum(-f(n + 1), (n, -tau, -1)) + Sum(f(n + 1), (n, -tau, T))
>>> Sum_step_backward(z, step=tau, minus=False)
Sum(f(n + 1), (n, 0, T - tau - 1)) + Sum(f(n + 1), (n, T - tau, T))
>>> Sum_step_backward(z, step=-tau, minus=True)
Sum(-f(n + 1), (n, T + 1, T + tau)) + Sum(f(n + 1), (n, 0, T + tau))
>>> z = Sum(f(n + m), (n, 0, T), (m, 0, tau))
>>> Sum_step_forward(z, where=-1) # default 'where'.
Sum(f(n), (n, 0, T)) + Sum(f(m + n), (n, 0, T), (m, 1, tau))
>>> Sum_step_forward(z, where=-2)
Sum(f(m) + Sum(f(m + n), (n, 1, T)), (m, 0, tau))

```

I intentionally omitted infinite checks, etc.

Mixed Example:

```python
>>> Mf = MatrixFunction("Mf", n, n)
>>> z = Sum(Mf(m), (m, 0, 2))
>>> Sum_step_forward(z, step=2)
Mf(0) + Mf(1) + Mf(2)
>>> z = Sum(Mf(m), (m, 0, T))
>>> z
Sum(Mf(m), (m, 0, T))
>>> # However, z is not correctly typed.
>>> z.is_Matrix
False

```

If you want something like above, you should use MatSum.


## Usage of MatSum and MatProduct (**Experimental**)

```python
>>> Mf = MatrixFunction("Mf", n, n)
>>> z = MatSum(Mf(m), (m, 0, 2))
>>> z
MatSum(Mf(m), (m, 0, 2))
>>> latex(z)
'\\sum_{m=0}^{2} \\operatorname{Mf}{\\left(m \\right)}'
>>> z = MatSum(MatSum(Mf(n + m), (m, 0, T)), (n, 0, tau))
>>> z
MatSum(Mf(m + n), (m, 0, T), (n, 0, tau))
>>> z = MatProduct(Mf(m), (m, 0, T))
>>> Product_step_forward(z)
Mf(0)*MatProduct(Mf(m), (m, 1, T))

```

## Tests (for developers)

```sh
$ python -m pytest -s
$ python -m doctest README.md -v
```

## Author

JRF ( http://jrf.cocolog-nifty.com/statuses )


## License

MIT License.

Note: Many parts are "quoted" from the SymPy sources.
